{
 "cells": [
  {
   "cell_type": "markdown",
   "metadata": {},
   "source": [
    "# Show Your Working - Trigonometry Two\n",
    "\n",
    "<hr>\n",
    "\n",
    "\n",
    "## Question 11\n",
    "<hr>\n",
    "Prove that:\n",
    "$$\\cos^4\\theta-\\sin^4\\theta+1=2\\cos^2\\theta$$\n",
    "## Question 12\n",
    "<hr>\n",
    "Prove that:\n",
    "$$\\tan\\theta\\mathrm{cosec}\\theta=\\sec\\theta$$\n",
    "## Question 13\n",
    "<hr>\n",
    "Prove that:\n",
    "$$\\frac{1}{\\sec^2\\theta}+\\frac{1}{\\mathrm{cosec}^2\\theta}=1$$\n",
    "## Question 14\n",
    "<hr>\n",
    "Prove that:\n",
    "$$\\sec\\theta-\\cos\\theta=\\sin\\theta\\tan\\theta$$\n",
    "## Question 15\n",
    "<hr>\n",
    "Prove that:\n",
    "$$\\mathrm{cosec}\\theta-\\sin\\theta=\\cot\\theta\\cos\\theta$$\n",
    "## Question 16\n",
    "<hr>\n",
    "Prove that:\n",
    "$$\\cos^2\\theta-\\sin^2\\theta=2\\cos^2\\theta-1$$\n",
    "## Question 17\n",
    "<hr>\n",
    "Prove that:\n",
    "$$\\sin^2\\theta+2\\cos^2\\theta=2-\\sin^2\\theta$$\n",
    "## Question 18\n",
    "<hr>\n",
    "Prove that:\n",
    "$$(\\sin\\theta+\\cos\\theta)^2-2\\sin\\theta\\cos\\theta=1$$\n",
    "## Question 19\n",
    "<hr>\n",
    "Prove that:\n",
    "$$\\sin^3\\theta+\\cos^3\\theta=(\\sin\\theta+\\cos\\theta)(1-\\sin\\theta\\cos\\theta)$$\n",
    "## Question 20\n",
    "<hr>\n",
    "Prove that:\n",
    "$$\\cos^2\\theta+3\\sin^2\\theta=3-2\\cos^2\\theta$$\n",
    "\n",
    "<br><hr><hr><br>\n",
    "\n",
    "## Answer to Question 11\n",
    "<hr>\n",
    "Proof:\n",
    "$$\\cos^4\\theta-\\sin^4\\theta+1$$<br>\n",
    "$$=\\cos^4\\theta-(\\sin^2\\theta)(\\sin^2\\theta)+1$$<br>\n",
    "$$=\\cos^4\\theta-(1-\\cos^2\\theta)(1-\\cos^2\\theta)+1$$<br>\n",
    "$$=\\cos^4\\theta-(\\cos^4\\theta-2\\cos\\theta+1)+1$$<br>\n",
    "$$=2\\cos^2\\theta$$<br>\n",
    "## Answer to Question 12\n",
    "<hr>\n",
    "Proof:\n",
    "$$\\tan\\theta\\mathrm{cosec}\\theta$$<br>\n",
    "$$=\\frac{\\sin\\theta}{\\cos\\theta}\\frac{1}{\\sin\\theta}$$<br>\n",
    "$$=\\frac{1}{\\cos\\theta}$$<br>\n",
    "$$=\\sec\\theta$$<br>\n",
    "## Answer to Question 13\n",
    "<hr>\n",
    "Proof:\n",
    "$$\\frac{1}{\\sec^2\\theta}+\\frac{1}{\\mathrm{cosec}^2\\theta}$$<br>\n",
    "$$=\\frac{1}{\\frac{1}{\\cos^2\\theta}}+\\frac{1}{\\frac{1}{\\sin^2\\theta}}$$<br>\n",
    "$$=\\cos^2\\theta+\\sin^2\\theta$$<br>\n",
    "$$=1$$<br>\n",
    "## Answer to Question 14\n",
    "<hr>\n",
    "Proof:\n",
    "$$\\sec\\theta-\\cos\\theta=\\sin\\theta\\tan\\theta$$<br>\n",
    "$$\\frac{1}{\\cos\\theta}-\\cos\\theta=\\sin\\theta\\frac{\\sin\\theta}{\\cos\\theta}$$<br>\n",
    "Taking the right-hand side of the equation.\n",
    "$$=\\frac{\\sin^2\\theta}{\\cos\\theta}$$<br>\n",
    "$$=\\frac{1-\\cos^2\\theta}{\\cos\\theta}$$<br>\n",
    "$$=\\frac{1}{\\cos\\theta}-\\frac{\\cos^2\\theta}{\\cos\\theta}$$<br>\n",
    "$$=\\frac{1}{\\cos\\theta}-\\cos\\theta$$<br>\n",
    "## Answer to Question 15\n",
    "<hr>\n",
    "Proof:\n",
    "$$\\mathrm{cosec}\\theta-\\sin\\theta=\\cot\\theta\\cos\\theta$$<br>\n",
    "$$\\frac{1}{\\sin\\theta}-\\sin\\theta=\\frac{\\cos\\theta}{\\sin\\theta}\\cos\\theta$$<br>\n",
    "Taking the right-hand side of the equation.\n",
    "$$=\\frac{\\cos^2\\theta}{\\sin\\theta}$$<br>\n",
    "$$=\\frac{1-\\sin^2\\theta}{\\sin\\theta}$$<br>\n",
    "$$=\\frac{1}{\\sin\\theta}-\\frac{\\sin^2\\theta}{\\sin\\theta}$$<br>\n",
    "$$=\\frac{1}{\\sin\\theta}-\\sin\\theta$$<br>\n",
    "## Answer to Question 16\n",
    "<hr>\n",
    "Using the identity:\n",
    "$$\\sin^2\\theta=1-\\cos^2\\theta$$<br>\n",
    "Proof:\n",
    "$$\\cos^2\\theta-\\sin^2\\theta$$<br>\n",
    "$$=\\cos^2\\theta-(1-\\cos^2\\theta)$$<br>\n",
    "$$=\\cos^2\\theta-1+\\cos^2\\theta$$<br>\n",
    "$$=2\\cos^2\\theta-1$$<br>\n",
    "## Answer to Question 17\n",
    "<hr>\n",
    "Using the identity:\n",
    "$$\\cos^2\\theta=1-\\sin^2\\theta$$<br>\n",
    "Proof:\n",
    "$$\\sin^2\\theta+2\\cos^2\\theta$$<br>\n",
    "$$=\\sin^2\\theta+2(1-\\sin^2\\theta)$$<br>\n",
    "$$=\\sin^2\\theta+2-2\\sin^2\\theta$$<br>\n",
    "$$=2-\\sin^2\\theta$$<br>\n",
    "## Answer to Question 18\n",
    "<hr>\n",
    "Proof:\n",
    "$$(\\sin\\theta+\\cos\\theta)^2-2\\sin\\theta\\cos\\theta$$<br>\n",
    "$$=\\sin^2\\theta+2\\cos\\theta\\sin\\theta+\\cos^2\\theta-2\\sin\\theta\\cos\\theta$$<br>\n",
    "$$=\\sin^2\\theta+\\cos^2\\theta$$<br>\n",
    "$$=1$$<br>\n",
    "## Answer to Question 19\n",
    "<hr>\n",
    "Proof:\n",
    "$$(\\sin\\theta+\\cos\\theta)(1-\\sin\\theta\\cos\\theta)$$<br>\n",
    "$$=\\sin\\theta+\\cos\\theta-(\\sin^2\\theta\\cos\\theta+\\sin\\theta\\cos^2\\theta)$$<br>\n",
    "$$=\\sin\\theta+\\cos\\theta-((1-\\cos^2\\theta)\\cos\\theta+\\sin\\theta(1-\\sin^2\\theta))$$<br>\n",
    "$$=\\sin\\theta+\\cos\\theta - \\cos\\theta + \\cos^3\\theta - \\sin\\theta + \\sin^3\\theta$$<br>\n",
    "$$=\\cos^3\\theta+\\sin^3\\theta$$<br>\n",
    "## Answer to Question 20\n",
    "<hr>\n",
    "Proof:\n",
    "$$\\cos^2\\theta+3\\sin^2\\theta$$<br>\n",
    "$$=\\cos^2\\theta + 3(1-\\cos^2\\theta)$$<br>\n",
    "$$=\\cos^2\\theta+3-3\\cos^2\\theta$$<br>\n",
    "$$=3-2\\cos^2\\theta$$<br>\n"
   ]
  }
 ],
 "metadata": {
  "kernelspec": {
   "display_name": "Python 3",
   "language": "python",
   "name": "python3"
  },
  "language_info": {
   "codemirror_mode": {
    "name": "ipython",
    "version": 3
   },
   "file_extension": ".py",
   "mimetype": "text/x-python",
   "name": "python",
   "nbconvert_exporter": "python",
   "pygments_lexer": "ipython3",
   "version": "3.5.1"
  }
 },
 "nbformat": 4,
 "nbformat_minor": 0
}
